Red.v
@@ -1,151 +1,153 @@
-Require Import Misc.
 Require Import List.
+Require Import Arith.
 Require Import Freevar.
-Require Import Term.
+Require Import Misc.
+Require Import Psatz.
+Require Import Star.
+Require Import Coq.Logic.Eqdep_dec.
 Require Import FEnv.
+Require Import STerm.
+Require Import Pretty.
+Require Import Inductive.
+
 
 Inductive nfval :=
-| NFFreeVar : freevar -> nfval
-| NFStructApp : nfval -> nfval_or_lam -> nfval
-| NFStructMatch : nfval -> list (list freevar * nfval_or_lam) -> nfval
+| nvar : nat -> nfval
+| napp : nfval -> nfval_or_lam -> nfval
+| nswitch : nfval -> list (nat * nfval_or_lam) -> nfval
 
 with nfval_or_lam :=
-| NFVal : nfval -> nfval_or_lam
-| NFLam : freevar -> nfval_or_lam -> nfval_or_lam
-| NFConstr : nat -> list nfval_or_lam -> nfval_or_lam.
+| nval : nfval -> nfval_or_lam
+| nlam : nfval_or_lam -> nfval_or_lam
+| nconstr : nat -> list nfval_or_lam -> nfval_or_lam.
 
-Inductive envitem :=
-| EVal : nfval -> envitem
-| ELazy : term -> envitem
-| ELam : term -> freevar -> envitem
-| EConstr : nat -> list freevar -> envitem.
+Inductive val : deep_flag -> Type :=
+| vals_nf : nfval -> val shallow
+| vals_abs : term -> val shallow
+| vals_constr : nat -> list term -> val shallow
+| vald_nf : nfval_or_lam -> val deep.
 
-Inductive cont :=
-| KNil : cont
-| KUpdateLazy : freevar -> list term -> cont -> cont
-| KUpdateLam : term -> freevar -> cont -> cont
-| KApp : nfval -> list term -> cont -> cont.
-
-Record state := mkState {
-  st_code : envitem ;
-  st_stack : list term ;
-  st_env : list (freevar * envitem) ;
-  st_cont : cont ;
-  st_lamnf : list (freevar * nfval_or_lam) ;
-  st_usedvars : list freevar ;
-}.
-
-Inductive red : state -> state -> Prop :=
-| red_app : forall t u e pi K W L,
-    red {| st_code := ELazy (app t u) ; st_stack := pi ; st_env := e ; st_cont := K ; st_lamnf := W ; st_usedvars := L |}
-        {| st_code := ELazy t ; st_stack := u :: pi ; st_env := e ; st_cont := K ; st_lamnf := W ; st_usedvars := L |}
-| red_lam : forall t e pi K W L y,
-    y \notin L ->
-    red {| st_code := ELazy (lam t) ; st_stack := pi ; st_env := e ; st_cont := K ; st_lamnf := W ; st_usedvars := L |}
-        {| st_code := ELam t y ; st_stack := pi ; st_env := e ; st_cont := K ; st_lamnf := W ; st_usedvars := y :: L |}
-| red_redex : forall t u e pi K W L x y,
-    x \notin L ->
-    red {| st_code := ELam t y ; st_stack := u :: pi ; st_env := e ; st_cont := K ; st_lamnf := W ; st_usedvars := L |}
-        {| st_code := ELazy (t ^ x) ; st_stack := pi ; st_env := (x, ELazy u) :: e ; st_cont := K ; st_lamnf := W ; st_usedvars := x :: L |}
-| red_var_open : forall x e pi K W L,
-    env_find e x = None ->
-    red {| st_code := ELazy (fvar x) ; st_stack := pi ; st_env := e ; st_cont := K ; st_lamnf := W ; st_usedvars := L |}
-        {| st_code := EVal (NFFreeVar x) ; st_stack := pi ; st_env := e ; st_cont := K ; st_lamnf := W ; st_usedvars := L |}
-| red_var_val : forall x e v pi K W L,
-    env_find e x = Some (EVal v) ->
-    red {| st_code := ELazy (fvar x) ; st_stack := pi ; st_env := e ; st_cont := K ; st_lamnf := W ; st_usedvars := L |}
-        {| st_code := EVal v ; st_stack := pi ; st_env := e ; st_cont := K ; st_lamnf := W ; st_usedvars := L |}
-| red_var_lazy : forall x e t pi K W L,
-    env_find e x = Some (ELazy t) ->
-    red {| st_code := ELazy (fvar x) ; st_stack := pi ; st_env := e ; st_cont := K ; st_lamnf := W ; st_usedvars := L |}
-        {| st_code := ELazy t ; st_stack := nil ; st_env := e ; st_cont := KUpdateLazy x pi K ; st_lamnf := W ; st_usedvars := L |}
-| red_var_lam : forall x e t y pi K W L,
-    env_find e x = Some (ELam t y) ->
-    red {| st_code := ELazy (fvar x) ; st_stack := pi ; st_env := e ; st_cont := K ; st_lamnf := W ; st_usedvars := L |}
-        {| st_code := ELam t y ; st_stack := pi ; st_env := e ; st_cont := K ; st_lamnf := W ; st_usedvars := L |}
-| red_app_val : forall v e u pi K W L,
-    red {| st_code := EVal v ; st_stack := u :: pi ; st_env := e ; st_cont := K ; st_lamnf := W ; st_usedvars := L |}
-        {| st_code := ELazy u ; st_stack := nil ; st_env := e ; st_cont := KApp v pi K ; st_lamnf := W ; st_usedvars := L |}
-| red_lam_deepen : forall t x e K W L,
-    env_find W x = None ->
-    red {| st_code := ELam t x ; st_stack := nil ; st_env := e ; st_cont := K ; st_lamnf := W ; st_usedvars := L |}
-        {| st_code := ELazy (t ^ x) ; st_stack := nil ; st_env := e ; st_cont := KUpdateLam t x K ; st_lamnf := W ; st_usedvars := L |}
-| red_cont_app_val : forall v1 v2 pi K e W L,
-    red {| st_code := EVal v1 ; st_stack := nil ; st_env := e ; st_cont := KApp v2 pi K ; st_lamnf := W ; st_usedvars := L |}
-        {| st_code := EVal (NFStructApp v2 (NFVal v1)) ; st_stack := pi ; st_env := e ; st_cont := K ; st_lamnf := W ; st_usedvars := L |}
-| red_cont_app_lam : forall t x body v pi K e W L,
-    env_find W x = Some body ->
-    red {| st_code := ELam t x ; st_stack := nil ; st_env := e ; st_cont := KApp v pi K ; st_lamnf := W ; st_usedvars := L |}
-        {| st_code := EVal (NFStructApp v (NFLam x body)) ; st_stack := pi ; st_env := e ; st_cont := K ; st_lamnf := W ; st_usedvars := L |}
-| red_cont_update_lam_val : forall t v x K e W L,
-    red {| st_code := EVal v ; st_stack := nil ; st_env := e ; st_cont := KUpdateLam t x K ; st_lamnf := W ; st_usedvars := L |}
-        {| st_code := ELam t x ; st_stack := nil ; st_env := e ; st_cont := K ; st_lamnf := (x, NFVal v) :: W ; st_usedvars := L |}
-| red_cont_update_lam_lam : forall t1 t2 y body x K e W L,
-    env_find W y = Some body ->
-    red {| st_code := ELam t2 y ; st_stack := nil ; st_env := e ; st_cont := KUpdateLam t1 x K ; st_lamnf := W ; st_usedvars := L |}
-        {| st_code := ELam t1 x ; st_stack := nil ; st_env := e ; st_cont := K ; st_lamnf := (x, NFLam y body) :: W ; st_usedvars := L |}
-| red_cont_update_lazy_val : forall v x pi e K W L,
-    red {| st_code := EVal v ; st_stack := nil ; st_env := e ; st_cont := KUpdateLazy x pi K ; st_lamnf := W ; st_usedvars := L |}
-        {| st_code := EVal v ; st_stack := pi ; st_env := update_env e x (EVal v) ; st_cont := K ; st_lamnf := W ; st_usedvars := L |}
-| red_cont_update_lazy_lam : forall t y x pi e K W L,
-    red {| st_code := ELam t y ; st_stack := nil ; st_env := e ; st_cont := KUpdateLazy x pi K ; st_lamnf := W ; st_usedvars := L |}
-        {| st_code := ELam t y ; st_stack := pi ; st_env := update_env e x (ELam t y) ; st_cont := K ; st_lamnf := W ; st_usedvars := L |}
-.
-
-Fixpoint read_nfval (v : nfval) :=
-  match v with
-  | NFFreeVar x => fvar x
-  | NFStructApp v1 v2 => app (read_nfval v1) (read_nfval_or_lam v2)
-  end
-
-with read_nfval_or_lam (v : nfval_or_lam) :=
-  match v with
-  | NFVal v => read_nfval v
-  | NFLam x v => lam (closeb 0 x (read_nfval_or_lam v))
-  end.
-
-Definition read_envitem (ei : envitem) :=
-  match ei with
-  | EVal v => read_nfval v
-  | ELam t x => lam t
-  | ELazy t => t
-  end.
-
-Fixpoint read_stack t pi :=
-  match pi with
-  | nil => t
-  | u :: pi => read_stack (app t u) pi
+Definition val_nf {df} v : val df :=
+  match df with
+  | shallow => vals_nf v
+  | deep => vald_nf (nval v)
   end.
 
 
-Fixpoint nfval_ind2 (P : nfval -> Prop) (Q : nfval_or_lam -> Prop)
-         (Hfree : forall x, P (NFFreeVar x)) (Happ : forall v1 v2, P v1 -> Q v2 -> P (NFStructApp v1 v2))
-         (Hval : forall v, P v -> Q (NFVal v)) (Hlam : forall x v, Q v -> Q (NFLam x v)) v : P v :=
-  match v with
-  | NFFreeVar x => Hfree x
-  | NFStructApp v1 v2 => Happ v1 v2 (nfval_ind2 P Q Hfree Happ Hval Hlam v1) (nfval_or_lam_ind2 P Q Hfree Happ Hval Hlam v2)
-  end
+Inductive ext : deep_flag -> Type :=
+| ext_term : forall df, term -> ext df
+| ext_app : forall df, out (val shallow) -> term -> ext df
+| ext_appnf : forall df, nfval -> out (val deep) -> ext df
+| ext_switch : forall df, out (val shallow) -> list (nat * term) -> ext df
+| ext_switchnf : forall df, nfval -> list (nat * nfval_or_lam) -> option (nat * out (val deep)) -> list (nat * term) -> ext df
+| extd_abs : out (val deep) -> ext deep
+| extd_constr : nat -> list nfval_or_lam -> option (out (val deep)) -> list term -> ext deep.
 
-with nfval_or_lam_ind2 (P : nfval -> Prop) (Q : nfval_or_lam -> Prop)
-         (Hfree : forall x, P (NFFreeVar x)) (Happ : forall v1 v2, P v1 -> Q v2 -> P (NFStructApp v1 v2))
-         (Hval : forall v, P v -> Q (NFVal v)) (Hlam : forall x v, Q v -> Q (NFLam x v)) v : Q v :=
-  match v with
-  | NFVal v => Hval v (nfval_ind2 P Q Hfree Happ Hval Hlam v)
-  | NFLam x v => Hlam x v (nfval_or_lam_ind2 P Q Hfree Happ Hval Hlam v)
+Arguments ext_term {df} _.
+Arguments ext_app {df} _ _.
+Arguments ext_appnf {df} _ _.
+Arguments ext_switch {df} _ _.
+Arguments ext_switchnf {df} _ _ _ _.
+
+Definition get_abort {df t} (e : ext df) : option (out t) :=
+  match e with
+  | ext_term _ => None
+  | ext_app o _ => get_out_abort o
+  | ext_appnf _ o => get_out_abort o
+  | ext_switch o _ => get_out_abort o
+  | ext_switchnf _ _ o _ => match o with Some (_, o) => get_out_abort o | None => None end
+  | extd_abs o => get_out_abort o
+  | extd_constr _ _ o _ => match o with Some o => get_out_abort o | None => None end
   end.
 
-Definition nfval_and_lam_ind2 P Q Hfree Happ Hval Hlam :=
-  conj (fun v => nfval_ind2 P Q Hfree Happ Hval Hlam v) (fun v => nfval_or_lam_ind2 P Q Hfree Happ Hval Hlam v).
+Inductive red_ (rec : forall df, ext df -> out (val df) -> Prop) : forall df, ext df -> out (val df) -> Prop :=
+| red_var : forall df n,
+    red_ rec df (ext_term (var n)) (out_ret (val_nf (nvar n))) (* Free variables reduce to themselves *)
+| red_abs_shallow : forall t,
+    red_ rec shallow (ext_term (abs t)) (out_ret (vals_abs t)) (* Do not look under abstractions *)
+| red_abs_deep : forall t o1 o2,
+    rec deep (ext_term t) o1 ->
+    rec deep (extd_abs o1) o2 ->
+    red_ rec deep (ext_term (abs t)) o2
+| red_abs1 : forall v,
+    red_ rec deep (extd_abs (out_ret (vald_nf v))) (out_ret (vald_nf (nlam v)))
+| red_app : forall df t1 o1 t2 o2,
+    rec shallow (ext_term t1) o1 ->
+    rec df (ext_app o1 t2) o2 ->
+    red_ rec df (ext_term (app t1 t2)) o2
+| red_app1_nf : forall df v o1 t2 o2,
+    rec deep (ext_term t2) o1 ->
+    rec df (ext_appnf v o1) o2 ->
+    red_ rec df (ext_app (out_ret (vals_nf v)) t2) o2
+| red_app1_abs : forall df t1 t2 o,
+    rec df (ext_term (subst1 t2 t1)) o ->
+    red_ rec df (ext_app (out_ret (vals_abs t1)) t2) o
+| red_appnf : forall df v1 v2,
+    red_ rec df (ext_appnf v1 (out_ret (vald_nf v2))) (out_ret (val_nf (napp v1 v2)))
+| red_constr_shallow : forall tag l,
+    red_ rec shallow (ext_term (constr tag l)) (out_ret (vals_constr tag l))
+| red_constr_deep : forall tag l o,
+    rec deep (extd_constr tag nil None l) o ->
+    red_ rec deep (ext_term (constr tag l)) o
+| red_constr1_done : forall tag l,
+    red_ rec deep (extd_constr tag l None nil) (out_ret (vald_nf (nconstr tag l)))
+| red_constr1_step1 : forall tag l1 l2 t o1 o2,
+    rec deep (ext_term t) o1 ->
+    rec deep (extd_constr tag l1 (Some o1) l2) o2 ->
+    red_ rec deep (extd_constr tag l1 None (t :: l2)) o2
+| red_constr1_step2 : forall tag l1 l2 v o,
+    rec deep (extd_constr tag (l1 ++ v :: nil) None l2) o ->
+    red_ rec deep (extd_constr tag l1 (Some (out_ret (vald_nf v))) l2) o
+| red_switch : forall df t o1 m o2,
+    rec shallow (ext_term t) o1 ->
+    rec df (ext_switch o1 m) o2 ->
+    red_ rec df (ext_term (switch t m)) o2
+| red_switch1_constr : forall df tag l m t o,
+    nth_error m tag = Some (length l, t) ->
+    rec df (ext_term (subst (read_env l) t)) o ->
+    red_ rec df (ext_switch (out_ret (vals_constr tag l)) m) o
+| red_switch1_nf : forall df v m o,
+    rec df (ext_switchnf v nil None m) o ->
+    red_ rec df (ext_switch (out_ret (vals_nf v)) m) o
+| red_switchnf_done : forall df v m,
+    red_ rec df (ext_switchnf v m None nil) (out_ret (val_nf (nswitch v m)))
+| red_switchnf_step1 : forall df v m1 m2 p t o1 o2,
+    rec deep (ext_term t) o1 ->
+    rec df (ext_switchnf v m1 (Some (p, o1)) m2) o2 ->
+    red_ rec df (ext_switchnf v m1 None ((p, t) :: m2)) o2
+| red_switchnf_step2 : forall df m1 m2 v1 v2 p o,
+    rec df (ext_switchnf v1 (m1 ++ (p, v2) :: nil) None m2) o ->
+    red_ rec df (ext_switchnf v1 m1 (Some (p, out_ret (vald_nf v2))) m2) o
+| red_abort : forall df e o,
+    get_abort e = Some o -> red_ rec df e o.
+
+Inductive red : forall df, ext df -> out (val df) -> Prop :=
+| mkred : forall df e o, red_ red df e o -> red df e o.
+
+CoInductive cored : forall df, ext df -> out (val df) -> Prop :=
+| mkcored : forall df e o, red_ cored df e o -> cored df e o.
+
+Lemma red_ind3 : is_ind3 red_ red.
+Proof. prove_ind3. Qed.
 
 
-Lemma nfval_and_lam_lc :
-  (forall v, lc (read_nfval v)) /\ (forall v, lc (read_nfval_or_lam v)).
+Lemma red_not_div_preserved_down :
+  preserved_down3 red_ red (fun df e o => o <> out_div).
 Proof.
-  apply nfval_and_lam_ind2.
-  - intros; simpl; constructor.
-  - intros; simpl; constructor; assumption.
-  - intros; simpl; assumption.
-  - intros; simpl. apply lc_lam_body. apply closeb_body. assumption.
+  intros df e o Q H1 H2.
+  inversion H1; unexistT; subst; unexistT; subst;
+    repeat (match goal with [ H : ?A /\ Q _ _ _ |- _ ] => destruct H end);
+    try (econstructor; (eassumption || tauto)).
+  - econstructor; splits 3; try eassumption.
+    intros ->. apply (ind3_inv _ _ red_ind3) in H0; inversion H0; unexistT; subst; simpl in *; autoinjSome; tauto.
+  - econstructor; splits 3; try eassumption.
+    intros ->. apply (ind3_inv _ _ red_ind3) in H; inversion H; unexistT; subst; simpl in *; autoinjSome; tauto.
+  - econstructor; splits 3; try eassumption.
+    intros ->. apply (ind3_inv _ _ red_ind3) in H; inversion H; unexistT; subst; simpl in *; autoinjSome; tauto.
+  - econstructor; splits 3; try eassumption.
+    intros ->. apply (ind3_inv _ _ red_ind3) in H0; inversion H0; unexistT; subst; simpl in *; autoinjSome; tauto.
+  - econstructor; splits 3; try eassumption.
+    intros ->. apply (ind3_inv _ _ red_ind3) in H; inversion H; unexistT; subst; simpl in *; autoinjSome; tauto.
+  - econstructor; splits 3; try eassumption.
+    intros ->. apply (ind3_inv _ _ red_ind3) in H; inversion H; unexistT; subst; simpl in *; autoinjSome; tauto.
 Qed.
-
-Definition nfval_or_lam_lc := proj2 nfval_and_lam_lc.
