Costar.v
@@ -1,0 +1,167 @@
+Require Import List.
+Require Import Arith.
+Require Import Freevar.
+Require Import Misc.
+Require Import Psatz.
+Require Import Star.
+Require Import Coq.Logic.Eqdep_dec.
+Require Import FEnv.
+Require Import STerm.
+Require Import Inductive.
+
+CoInductive infred {A : Type} (R : A -> A -> Prop) : A -> Prop :=
+| infred_step : forall x y, R x y -> infred R y -> infred R x.
+CoInductive costar {A : Type} (R : A -> A -> Prop) : A -> option A -> Prop :=
+| costar_refl : forall x, costar R x (Some x)
+| costar_step : forall x y z, R x y -> costar R y z -> costar R x z.
+Definition costarP {A : Type} (R : A -> A -> Prop) x y :=
+  exists H, H x y /\ forall x1 y1, H x1 y1 -> y1 = Some x1 \/ exists z, R x1 z /\ H z y1.
+
+Lemma costarP_costar :
+  forall A (R : A -> A -> Prop) x y, costarP R x y -> costar R x y.
+Proof.
+  intros A R. cofix IH. intros x y (H & H1 & H2).
+  apply H2 in H1. destruct H1 as [H1 | (z & HR & H1)].
+  - subst. constructor.
+  - econstructor; [eassumption|]. apply IH. exists H; split; assumption.
+Qed.
+
+Lemma infred_map_impl :
+  forall (A B : Type) (RA : A -> A -> Prop) (RB : B -> B -> Prop) (f : A -> B),
+    (forall x y : A, RA x y -> RB (f x) (f y)) -> forall x : A, infred RA x -> infred RB (f x).
+Proof.
+  intros A B RA RB f H. cofix IH. intros x Hx. inversion Hx; subst.
+  econstructor; [apply H; eassumption|].
+  apply IH. assumption.
+Qed.
+
+Lemma costar_map_impl :
+  forall (A B : Type) (RA : A -> A -> Prop) (RB : B -> B -> Prop) (f : A -> B),
+    (forall x y : A, RA x y -> RB (f x) (f y)) ->
+    forall x y, costar RA x y -> costar RB (f x) (match y with None => None | Some y => Some (f y) end).
+Proof.
+  intros A B RA RB f H. cofix IH. intros x y Hx. inversion Hx; subst.
+  - constructor.
+  - econstructor; [apply H; eassumption|].
+    apply IH. assumption.
+Qed.
+
+Lemma costar_compose :
+  forall (A : Type) (R : A -> A -> Prop) x y z,
+    costar R x y -> (forall w, y = Some w -> costar R w z) -> costar R x z.
+Proof.
+  intros A R. cofix IH. intros x y z H1 H2. inversion H1; subst.
+  - apply H2. reflexivity.
+  - econstructor; [eassumption|].
+    eapply IH; eassumption.
+Defined.
+
+Definition weaken {A : Type} (x y : A * nat) := fst x = fst y /\ snd y <= snd x.
+Definition weakenO {A : Type} (x y : option (A * nat)) := match x, y with None, None => True | Some x, Some y => weaken x y | _, _ => False end.
+
+Lemma weaken_refl : forall (A : Type) (x : A * nat), weaken x x.
+Proof.
+  intros A [x y]. unfold weaken. simpl. split; reflexivity.
+Qed.
+
+Lemma weakenO_refl : forall (A : Type) (x : option (A * nat)), weakenO x x.
+Proof.
+  intros A [x|]; unfold weakenO; simpl.
+  - apply weaken_refl.
+  - tauto.
+Qed.
+
+Definition stepped {A : Type} (R : A -> A -> Prop) x y := R (fst x) (fst y) \/ (fst x = fst y /\ snd y < snd x).
+
+Definition costarPTn {A : Type} (R : A -> A -> Prop) x y :=
+  exists H, H x y /\ forall x1 y1, H x1 y1 ->
+                        weakenO (Some x1) y1 \/
+                        (exists z1, stepped R x1 z1 /\ H z1 y1) \/
+                        (exists z1 z2, stepped R x1 z1 /\ H z1 z2 /\ (forall v, z2 = Some v -> H v y1)).
+
+Lemma costarPTn_destruct :
+  forall (A : Type) (R : A -> A -> Prop) x y,
+    costarPTn R x y -> weakenO (Some x) y \/
+                      (exists z, stepped R x z /\ costarPTn R z y) \/
+                      (exists z1 z2, stepped R x z1 /\ costarPTn R z1 z2 /\ (forall v, z2 = Some v -> costarPTn R v y)).
+Proof.
+  intros A R x y (H & H1 & H2).
+  apply H2 in H1. destruct H1 as [H1 | [(z & Hz1 & Hz2) | (z1 & z2 & Hz1 & Hz2 & Hz3)]].
+  - left. assumption.
+  - right. left. exists z. split; [assumption|]. exists H; split; assumption.
+  - right. right. exists z1. exists z2. split; [assumption|]. split.
+    + exists H; split; assumption.
+    + intros v ->. exists H; split; [|assumption]. apply Hz3. reflexivity.
+Qed.
+
+Lemma weaken_trans :
+  forall (A : Type) (x y z : A * nat), weaken x y -> weaken y z -> weaken x z.
+Proof.
+  intros A [x1 x2] [y1 y2] [z1 z2]; unfold weaken; simpl.
+  intros [? ?] [? ?]; split; [congruence|lia].
+Qed.
+
+Lemma stepped_weaken :
+  forall (A : Type) (R : A -> A -> Prop) x y z, weaken x y -> stepped R y z -> stepped R x z.
+Proof.
+  intros A R [x1 x2] [y1 y2] [z1 z2] [H1 H2] [H3 | [H3 H4]]; simpl in *; subst.
+  - left; simpl; assumption.
+  - right; simpl; split; [reflexivity|lia].
+Qed.
+
+Lemma costarPTn_comp :
+  forall (A : Type) (R : A -> A -> Prop) x y z, costarPTn R x y -> (forall v, y = Some v -> costarPTn R v z) -> costarPTn R x z.
+Proof.
+  intros A R x y z H1 H2. exists (fun x1 y1 => costarPTn R x1 y1 \/ exists w, costarPTn R x1 w /\ (forall v, w = Some v -> costarPTn R v y1)).
+  split.
+  - right. exists y. split; assumption.
+  - clear x y z H1 H2. intros x z [Hxz | (y & Hxy & Hyz)].
+    + apply costarPTn_destruct in Hxz. destruct Hxz as [Hxz | [(z1 & Hz1 & Hz2) | (z1 & z2 & Hz1 & Hz2 & Hz3)]].
+      * left. assumption.
+      * right. left. exists z1. split; tauto.
+      * right. right. exists z1. exists z2. split; [assumption|]. split; [tauto|]. intros v Hv; left; apply Hz3; assumption.
+    + apply costarPTn_destruct in Hxy. destruct Hxy as [Hxy | [(z1 & Hz1 & Hz2) | (z1 & z2 & Hz1 & Hz2 & Hz3)]].
+      * destruct y as [y|]; simpl in *; [|tauto].
+        specialize (Hyz y eq_refl).
+        apply costarPTn_destruct in Hyz. destruct Hyz as [Hyz | [(z1 & Hz1 & Hz2) | (z1 & z2 & Hz1 & Hz2 & Hz3)]].
+        -- destruct z as [z|]; simpl in *; [|tauto].
+           left. eapply weaken_trans; eassumption.
+        -- right. left. exists z1. split; [eapply stepped_weaken; eassumption|].
+           left; assumption.
+        -- right. right. exists z1. exists z2. split; [eapply stepped_weaken; eassumption|].
+           split; [left; assumption|]. intros; left; apply Hz3; assumption.
+      * right. left. exists z1. split; [assumption|].
+        right. exists y. split; assumption.
+      * right. right. exists z1. exists z2. split; [assumption|].
+        split.
+        -- left; assumption.
+        -- intros v ->. right. exists y. split; [apply Hz3; reflexivity|].
+           intros w ->. apply Hyz. reflexivity.
+Qed.
+
+
+Lemma costarPTn_costarP :
+  forall (A : Type) (R : A -> A -> Prop) x y, costarPTn R x y -> costarP R (fst x) (option_map fst y).
+Proof.
+  intros A R x y H. exists (fun u v => exists n m, costarPTn R (u, n) (option_map (fun v => (v, m)) v)).
+  split.
+  - exists (snd x). exists (match y with Some y => snd y | None => 0 end).
+    destruct x as [x1 x2]. destruct y as [[y1 y2]|]; simpl; assumption.
+  - clear x y H. intros x y (n & m & H).
+    revert x y m H; induction n as [n Hn] using lt_wf_ind; intros x y m H.
+    apply costarPTn_destruct in H. destruct H as [H | [(z & Hz1 & Hz2) | (z1 & z2 & Hz1 & Hz2 & Hz3)]].
+    + destruct y as [y|]; simpl in H; [|tauto].
+      unfold weaken in H; simpl in H. left. destruct H; congruence.
+    + destruct Hz1 as [Hz1 | Hz1]; simpl in Hz1.
+      * right. exists (fst z). split; [assumption|].
+        exists (snd z). exists m. destruct z; assumption.
+      * destruct Hz1 as [-> Hz1]. destruct z as [z1 z2]; simpl in *.
+        eapply Hn; [|eassumption]. assumption.
+    + destruct Hz1 as [Hz1 | Hz1]; simpl in Hz1.
+      * right. exists (fst z1). split; [assumption|].
+        exists (snd z1). exists m. eapply costarPTn_comp; [destruct z1; simpl in *; eassumption|].
+        eassumption.
+      * destruct Hz1 as [-> Hz1]. destruct z1 as [z3 z4]; simpl in *.
+        eapply Hn; [exact Hz1|].
+        eapply costarPTn_comp; eassumption.
+Qed.
