Pretty.v
@@ -1,0 +1,32 @@
+
+Inductive out t :=
+| out_ret : t -> out t
+| out_div : out t.
+
+Arguments out_ret {t} _.
+Arguments out_div {t}.
+
+Definition out_map {A B : Type} (f : A -> B) (o : out A) : out B :=
+  match o with
+  | out_ret x => out_ret (f x)
+  | out_div => out_div
+  end.
+
+Definition get_out_abort {t1 t2} (o : out t1) : option (out t2) :=
+  match o with
+  | out_div => Some out_div
+  | _ => None
+  end.
+
+Lemma get_out_abort_div :
+  forall t1 t2 (o1 : out t1) (o2 : out t2), get_out_abort o1 = Some o2 -> o2 = out_div.
+Proof.
+  intros; destruct o1; simpl in *; congruence.
+Qed.
+
+Inductive outM t m :=
+| outM_ret : t -> m -> outM t m
+| outM_div : outM t m.
+
+Arguments outM_ret {t} {m} _ _.
+Arguments outM_div {t} {m}.
