RedEProof.v
@@ -1,0 +1,261 @@
+Require Import List.
+Require Import Arith.
+Require Import Freevar.
+Require Import Misc.
+Require Import Psatz.
+Require Import Star.
+Require Import Coq.Logic.Eqdep_dec.
+Require Import FEnv.
+Require Import STerm.
+Require Import Red.
+Require Import RedE.
+Require Import Pretty.
+Require Import Inductive.
+
+Fixpoint index l x :=
+  match l with
+  | nil => 0
+  | y :: l => if freevar_eq_dec x y then 0 else S (index l x)
+  end.
+
+Fixpoint read_clo (xs : list freevar) (c : clo) : term :=
+  match c with
+  | clo_var x => var (index xs x)
+  | clo_term _ t l =>
+    let nl := map (read_clo xs) l in
+    subst (read_env nl) t
+  end.
+
+Lemma read_shift_clo :
+  forall c x xs, x \notin clo_fv c -> clo_closed c -> read_clo (x :: xs) c = ren_term (plus_ren 1) (read_clo xs c).
+Proof.
+  induction c using clo_ind2; intros y ys Hy Hcc; inversion Hcc; subst; simpl in *.
+  - f_equal. destruct freevar_eq_dec; [tauto|]. lia.
+  - rewrite ren_subst. eapply subst_closed_at_ext; [eassumption|].
+    intros n Hn. unfold comp, read_env.
+    rewrite !nth_error_map.
+    destruct nth_error as [u|] eqn:Hu; [|apply nth_error_None in Hu; lia].
+    assert (u \in l) by (eapply nth_error_In; eassumption).
+    rewrite Forall_forall in H. apply H; [eassumption| |apply H4; assumption].
+    rewrite concat_map_In in Hy. intros Hy2; apply Hy; exists u; tauto.
+Qed.
+
+Fixpoint read_nfvalx xs v :=
+  match v with
+  | nxvar x => nvar (index xs x)
+  | nxapp v1 v2 => napp (read_nfvalx xs v1) (read_nfvalx_or_lam xs v2)
+  | nxswitch t m => nswitch (read_nfvalx xs t) (map (fun pt2 => (length (fst pt2), read_nfvalx_or_lam (fst pt2 ++ xs) (snd pt2))) m)
+  end
+
+with read_nfvalx_or_lam xs v :=
+  match v with
+  | nxval v => nval (read_nfvalx xs v)
+  | nxlam x v => nlam (read_nfvalx_or_lam (x :: xs) v)
+  | nxconstr tag l => nconstr tag (map (read_nfvalx_or_lam xs) l)
+  end.
+
+Definition read_valE {df} (xs : list freevar) (v : valE df) : val df :=
+  match v with
+  | valE_nf v => val_nf (read_nfvalx xs v)
+  | valEs_abs t l =>
+    vals_abs (subst (scons (var 0) (read_env (map (fun c => ren_term (plus_ren 1) (read_clo xs c)) l))) t)
+  | valEd_abs t l v => vald_nf (read_nfvalx_or_lam xs v)
+  | valEs_constr tag l =>
+    vals_constr tag (map (read_clo xs) l)
+  | valEd_constr tag l v => vald_nf (read_nfvalx_or_lam xs v)
+  end.
+
+Definition read_extE {df} xs (e : extE df) : ext df :=
+  match e with
+  | extE_term env t => ext_term (read_clo xs (clo_term xs t env))
+  | extE_clo c => ext_term (read_clo xs c)
+  | extE_app env o1 t2 => ext_app (out_map (read_valE xs) o1) (read_clo xs (clo_term xs t2 env))
+  | extE_appnf env v1 o2 => ext_appnf (read_nfvalx xs v1) (out_map (read_valE xs) o2)
+  | extE_switch env o m =>
+    ext_switch
+      (out_map (read_valE xs) o)
+      (map (fun pt2 => (fst pt2, subst (liftn_subst (fst pt2) (read_env (map (read_clo xs) env))) (snd pt2))) m)
+  | extE_switchnf1 env v m1 m2 =>
+    ext_switchnf
+      (read_nfvalx xs v)
+      (map (fun pt2 => (length (fst pt2), read_nfvalx_or_lam (fst pt2 ++ xs) (snd pt2))) m1)
+      None
+      (map (fun pt2 => (fst pt2, subst (liftn_subst (fst pt2) (read_env (map (read_clo xs) env))) (snd pt2))) m2)
+  | extE_switchnf2 env v m1 xs2 o m2 =>
+    ext_switchnf
+      (read_nfvalx xs v)
+      (map (fun pt2 => (length (fst pt2), read_nfvalx_or_lam (fst pt2 ++ xs) (snd pt2))) m1)
+      (Some (length xs2, out_map (read_valE (xs2 ++ xs)) o))
+      (map (fun pt2 => (fst pt2, subst (liftn_subst (fst pt2) (read_env (map (read_clo xs) env))) (snd pt2))) m2)
+  | extEd_abs env x t o => extd_abs (out_map (read_valE (x :: xs)) o)
+  | extEd_constr1 tag l l1 l2 =>
+    extd_constr tag
+                (map (read_nfvalx_or_lam xs) l1)
+                None
+                (map (read_clo xs) l2)
+  | extEd_constr2 tag l l1 o l2 =>
+    extd_constr tag
+                (map (read_nfvalx_or_lam xs) l1)
+                (Some (out_map (read_valE xs) o))
+                (map (read_clo xs) l2)
+  end.
+
+Lemma read_valE_deep :
+  forall (v : valE deep) xs, read_valE xs v = vald_nf (read_nfvalx_or_lam xs (getvalEd_nf v)).
+Proof.
+  intros v xs.
+  destruct (destruct_valE_deep v) as [[(v2 & ->) | (t & env & v2 & ->)] | (tag & l & v2 & ->)]; reflexivity.
+Qed.
+
+Lemma index_app :
+  forall L1 L2 x, x \in L1 -> index (L1 ++ L2) x = index L1 x.
+Proof.
+  intros L1 L2 x H. induction L1; simpl in *.
+  - tauto.
+  - destruct freevar_eq_dec; [reflexivity|]. f_equal. apply IHL1. destruct H; [congruence|tauto].
+Qed.
+
+Lemma index_app2 :
+  forall L1 L2 x, x \notin L1 -> index (L1 ++ L2) x = length L1 + index L2 x.
+Proof.
+  intros L1 L2 x H. induction L1; simpl in *.
+  - reflexivity.
+  - destruct freevar_eq_dec; subst; [simpl in *; tauto|]. f_equal.
+    apply IHL1. tauto.
+Qed.
+
+
+Lemma nth_error_index :
+  forall L p xs n x, distinct L p xs -> nth_error xs n = Some x -> index xs x = n.
+Proof.
+  intros L p xs n x H; revert n x; induction H; intros [|k] y Hy; simpl in *.
+  - congruence.
+  - congruence.
+  - destruct freevar_eq_dec; [reflexivity|]. congruence.
+  - destruct freevar_eq_dec; [|f_equal; apply IHdistinct; assumption].
+    subst. exfalso. eapply distinct_distinct; [eassumption|left; reflexivity|eapply nth_error_In; eassumption].
+Qed.
+
+Lemma read_shiftn_clo :
+  forall c ys p xs, distinct (clo_fv c) p ys -> clo_closed c -> read_clo (ys ++ xs) c = ren_term (plus_ren p) (read_clo xs c).
+Proof.
+  induction c using clo_ind2; intros ys p zs Hdistinct Hcc; inversion Hcc; subst; simpl in *.
+  - f_equal. erewrite index_app2, plus_ren_correct, distinct_length; [reflexivity|eassumption|].
+    intros H. eapply distinct_distinct; try eassumption. simpl. tauto.
+  - rewrite ren_subst. eapply subst_closed_at_ext; [eassumption|].
+    intros n Hn. unfold comp, read_env.
+    rewrite !nth_error_map.
+    destruct nth_error as [u|] eqn:Hu; [|apply nth_error_None in Hu; lia].
+    assert (u \in l) by (eapply nth_error_In; eassumption).
+    rewrite Forall_forall in H. apply H; [eassumption| |apply H4; assumption].
+    eapply distinct_incl; [|eassumption].
+    intros y Hy. rewrite concat_map_In. exists u. tauto.
+Qed.
+
+Lemma redE_red :
+  forall df xs dom fvs e o, redE df xs dom fvs e o -> fvs \subseteq xs /\ extE_closed_at e fvs -> forall fvs2, fvs \subseteq fvs2 -> red df (read_extE fvs2 e) (out_map (read_valE fvs2) o).
+Proof.
+  refine (preserved_with_inv6_rec _ _ redE_is_ind6 _ _ closed_preserved_down _).
+  intros df xs dom fvs e o H [Hfvs He] fvs2 Hfvs2. inversion H; unexistT; subst; unexistT; subst; simpl in *.
+  - apply H7.
+    rewrite <- Hfvs2. apply list_inter_subl2.
+  - constructor. constructor.
+  - unfold read_env. rewrite nth_error_map, H6.
+    apply H7. assumption.
+  - inversion He; subst. inversion H6; subst.
+    erewrite subst_closed_at_ext; [constructor; constructor|eassumption|].
+    intros [|n] Hn; [reflexivity|]. simpl; unfold read_env, comp; simpl.
+    rewrite !nth_error_map; destruct nth_error as [u|] eqn:Hu.
+    + reflexivity.
+    + apply nth_error_None in Hu. lia.
+  - inversion He; subst. inversion H7; subst.
+    constructor; econstructor; [|apply H11; assumption].
+    erewrite subst_closed_at_ext.
+    + eapply H10. rewrite Hfvs2; reflexivity.
+    + eassumption.
+    + intros [|n] Hn; simpl; unfold comp, read_env; simpl; [destruct freevar_eq_dec; congruence|].
+      rewrite !nth_error_map; destruct nth_error as [u|] eqn:Hu; [|apply nth_error_None in Hu; lia].
+      apply nth_error_In, H5 in Hu. destruct Hu as [Hu1 Hu2].
+      rewrite read_shift_clo; [reflexivity| |apply Hu1].
+      rewrite Hu2, Hfvs. assumption.
+  - rewrite read_valE_deep. constructor; constructor.
+  - constructor; econstructor; [eapply H6|eapply H7]; assumption.
+  - constructor; econstructor; [eapply H6|eapply H7]; assumption.
+  - inversion He; subst. inversion H10; subst.
+    constructor; econstructor.
+    unfold subst1. rewrite subst_subst.
+    erewrite subst_closed_at_ext; [eapply H8| |].
+    + assumption.
+    + eassumption.
+    + unfold comp, read_env.
+      intros [|n] Hn; simpl.
+      * destruct t2; try reflexivity. simpl.
+        rewrite nth_error_map. destruct nth_error eqn:Hu; [|apply nth_error_None in Hu; inversion H9; subst; lia].
+        reflexivity.
+      * rewrite !nth_error_map; destruct nth_error as [u|] eqn:Hu; [|apply nth_error_None in Hu; lia].
+        rewrite subst_ren; unfold comp; simpl.
+        erewrite subst_ext; [apply subst_id|]; intros; f_equal; lia.
+  - rewrite read_valE_deep. constructor; constructor.
+  - replace (map (read_clo fvs2) lc) with (map (subst (read_env (map (read_clo fvs2) env))) l); [constructor; constructor|].
+    eapply Forall2_map_eq, Forall2_impl; [|eassumption]. intros t c Htc; simpl in *.
+    destruct env_get_maybe_var as [c1|] eqn:Hc1.
+    + subst. destruct t; simpl in *; try congruence.
+      unfold read_env. rewrite nth_error_map, Hc1. reflexivity.
+    + destruct Htc as (xs2 & Hxs2a & Hxs2b & ->). reflexivity.
+  - constructor. constructor.
+    replace (map (subst (read_env (map (read_clo fvs2) env))) l) with (map (read_clo fvs2) lc).
+    + eapply H9. assumption.
+    + symmetry. eapply Forall2_map_eq, Forall2_impl; [|eassumption]. intros t c Htc; simpl in *.
+      destruct env_get_maybe_var as [c1|] eqn:Hc1.
+      * subst. destruct t; simpl in *; try congruence.
+        unfold read_env. rewrite nth_error_map, Hc1. reflexivity.
+      * destruct Htc as (xs2 & Hxs2a & Hxs2b & ->). reflexivity.
+  - constructor. constructor.
+  - constructor; econstructor; [apply H7; assumption|apply H9; assumption].
+  - rewrite read_valE_deep. constructor. econstructor.
+    rewrite <- map_app with (f := read_nfvalx_or_lam fvs2) (l' := getvalEd_nf v :: nil).
+    apply H5. assumption.
+  - constructor. econstructor.
+    + apply H6. assumption.
+    + apply H7. assumption.
+  - inversion He; subst.
+    constructor; econstructor; [rewrite nth_error_map, H6, map_length; simpl; reflexivity|].
+    rewrite subst_subst.
+    erewrite subst_closed_at_ext; [apply H7; assumption|eapply H8, nth_error_In; eassumption|].
+    intros n Hn. unfold comp, liftn_subst, read_env.
+    destruct le_lt_dec.
+    + rewrite !nth_error_map, nth_error_app2 by assumption.
+      destruct (nth_error env _) as [c|] eqn:Hc; [|apply nth_error_None in Hc; lia].
+      rewrite subst_ren. erewrite subst_ext; [apply subst_id|]. intros n2. simpl.
+      unfold comp; simpl. rewrite nth_error_map, plus_ren_correct, map_length.
+      replace (nth_error l (length l + n2)) with (@None clo) by (symmetry; apply nth_error_None; lia).
+      f_equal. lia.
+    + simpl. rewrite !nth_error_map, nth_error_app1 by assumption.
+      destruct (nth_error l _) as [c|] eqn:Hc; [|apply nth_error_None in Hc; lia]. reflexivity.
+  - constructor. constructor. apply H6. assumption.
+  - constructor. constructor.
+  - inversion He; subst.
+    constructor. econstructor.
+    + erewrite subst_closed_at_ext; [apply H8; rewrite Hfvs2; reflexivity|apply H13; left; reflexivity|].
+      intros n Hn. unfold liftn_subst, read_env.
+      destruct le_lt_dec.
+      * rewrite !nth_error_map, nth_error_app2 by (erewrite map_length, distinct_length; eassumption).
+        erewrite !map_length, app_length, map_length, distinct_length by eassumption.
+        destruct nth_error eqn:Hu.
+        -- erewrite read_shiftn_clo; [reflexivity| |eapply H7, nth_error_In; eassumption].
+           eapply distinct_incl; [|eassumption].
+           rewrite <- Hfvs. eapply H7, nth_error_In; eassumption.
+        -- apply nth_error_None in Hu. lia.
+      * rewrite nth_error_map, nth_error_app1, nth_error_map by (erewrite map_length, distinct_length; eassumption).
+        destruct nth_error as [y|] eqn:Hy.
+        -- simpl. f_equal. rewrite index_app; [|eapply nth_error_In; eassumption].
+           symmetry; eapply nth_error_index; eassumption.
+        -- apply nth_error_None in Hy. erewrite distinct_length in Hy by eassumption. lia.
+    + replace p with (length ys) by (eapply distinct_length; eassumption).
+      apply H9. assumption.
+  - rewrite read_valE_deep. constructor. econstructor.
+    rewrite <- map_app with (f := fun pt2 => (length (fst pt2), read_nfvalx_or_lam (fst pt2 ++ fvs2) (snd pt2))) (l' := (ys, getvalEd_nf v2) :: nil).
+    apply H6. assumption.
+  - constructor. constructor.
+    destruct e; simpl in *; try congruence; try (destruct o0; simpl in *; autoinjSome; simpl; congruence).
+Qed.
